Add examples

src/Lambda.v
@@ -1,39 +1,61 @@
 Require Import Monads.Tactics.
 Require Import Monads.Utils.
-Require Import Monads.DelayMonad.
+
 From Coq Require Import List Lia Arith.
 
 CoInductive Computation (A:Type) : Type :=
 | Return : A -> Computation A
-| Bind : forall (B:Type), Computation B-> (B-> Computation A)-> Computation A.
+| Bind : forall (B:Type), Computation B-> (B-> Computation A)-> Computation A
+| Fail
+| Step : Computation A -> Computation A.
 Arguments Return {A}.
 Arguments Bind {A B}.
-Notation "c >>= f" := (Bind c f) (at level 20).
+Arguments Step {A}.
+Arguments Fail {A}.
+
+Axiom Bind_On_Return: forall (A B: Type) (x: A) (f: A -> Computation B), 
+Bind (Return x) f = f x.
+
+Axiom Bind_On_Step: forall (A B: Type) (f: A -> Computation B) (x: Computation A), 
+Bind (Step x) f = Step (Bind x f).
+
 Notation "var <- c ; rest" :=
 (Bind c (fun var => rest) )
 (at level 60, right associativity).
 
-
-Definition OptPartial (A: Type):= Partial (option A).
-Definition fail {A: Type}:= rtrn (@None A).
-Print fail.
-
-Definition ret {A: Type}(x: A):= rtrn (Some x).
-Print ret.
-
-CoFixpoint bind {A B: Type}(x: OptPartial A) (f: A -> OptPartial B): OptPartial B :=
+Definition frob {A}(x: Computation A) :=
 match x with 
-| rtrn None => fail
-| rtrn (Some x) => f x
-| step y => step (bind y f) end.
+| Return y => Return y
+| Bind y f => Bind y f
+| Fail     => Fail
+| Step t   => Step t end.
 
-Notation "var <-- c ;; rest" :=
-(bind c (fun var => rest) )
-(at level 60, right associativity).
+Lemma frob_eq {A}: forall (x: Computation A), x = frob x.
+Proof. destruct x; reflexivity. Qed.
+
+CoInductive bisim {A} : Computation A -> Computation A -> Prop :=
+| BisimRtrn : forall x, bisim (Return x) (Return x)
+| BisimBind : forall (B: Type) (f: B -> Computation A) x, bisim (Bind x f) (Bind x f)
+| BisimStep : forall x y, bisim x y -> bisim (Step x) (Step y)
+| BisimStepL : forall x y, bisim x y -> bisim (Step x) y
+| BisimStepR : forall x y, bisim x y -> bisim x (Step y)
+| BisimFail: bisim Fail Fail.
+
+Theorem bisim_refl {A}: forall (a: Computation A), bisim a a.
+Proof. cofix CIH. intros. destruct a; constructor.
+- apply CIH. Qed.
+
+Theorem bisim_symm {A}: forall (a b: Computation A), bisim a b -> bisim b a.
+Proof. cofix CIH. intros. inversion H; subst; constructor. inversion H; 
+repeat (apply CIH in H0; assumption;
+  apply CIH in H0; assumption).
+apply CIH in H0; assumption. apply CIH in H0; assumption. Qed.
 
 
-Definition CompPartial (A: Type) := Computation (OptPartial A).
-Parameter const: Type.
+Theorem bisim_trans {A}: forall (a b c: Computation A), bisim a b -> bisim b c -> bisim a c.
+Proof. Admitted.
+
+Definition const :=nat. 
 
 Inductive term: Type :=
   | Var: nat -> term
@@ -46,27 +68,66 @@ Inductive value: Type :=
   | Clos: term -> list value -> value.
 
 Definition env := list value.
-Definition Fail {A: Type}:= Return (@fail A).
 
-
-Definition Ret {A: Type}(x: A):= Return (ret x).
-Print Ret.
-
-Definition demonad {A: Type} (x: CompPartial A):=
-match x with 
-| Return t => t
-| _ => fail end.
-
-CoFixpoint bs (t: term) (e:env): (CompPartial value) :=
+CoFixpoint bs (t: term) (e:env): (Computation value) :=
 match t with 
- | Const i => Ret (Int i)
+ | Const i => Return (Int i)
  | Var n   => match (nth_error e n) with 
-           | Some v => Ret v
+           | Some v => Return v
            | None   => Fail end
- | Fun a => Ret (Clos a e) 
- | App a b => op1 <- bs a e ; op2 <- bs b e ; 
-                        Return (v1 <-- op1 ;; v2 <-- op2 ;; match v1 with 
-                                    | Int n    => fail 
-                                    | Clos x y => fail end)
-                                                   end.
+ | Fun a => Return (Clos a e) 
+ | App a b => v1 <- bs a e ; v2 <- bs b e ; match v1 with 
+                                    | Int n    => Fail 
+                                    | Clos x y => Step (bs x (v2::y))
+                                                   end end.
+
+CoFixpoint never := @Step value never.
+
+Lemma bisim_successful: forall e, bisim ( bs (Const 2) e) (Return (Int 2)).
+Proof. intros. rewrite frob_eq with (x:=bs (Const 2) e). simpl. constructor. Qed.
+
+Lemma bisim_fail: forall e, bisim (bs (App (Const 1) (Const 2)) e) Fail.
+Proof. intros. rewrite frob_eq with (x:=bs (App (Const 1) (Const 2)) e). simpl. 
+rewrite frob_eq with (x:=bs (Const 1) e). rewrite frob_eq with (x:=bs (Const 2) e).
+simpl. rewrite Bind_On_Return. rewrite Bind_On_Return. constructor. Qed.
+
+Definition delta := Fun (App (Var 0) (Var 0)).
+Definition omega := App delta delta.
+
+Lemma delta_sim: forall e, (bisim (bs omega e)  
+(Step (bs (App (Var 0) (Var 0)) (Clos (App (Var 0) (Var 0)) e :: e)))).
+Proof. Admitted.
+
+Lemma bisim_infinite: forall e, bisim (bs omega e) never.
+Proof. cofix CIH. intros. rewrite frob_eq with (x:=bs omega e). simpl. 
+rewrite frob_eq with (x:=bs delta e). simpl. rewrite Bind_On_Return. 
+rewrite Bind_On_Return. constructor. 
+assert (bisim (bs omega e) (bs (App (Var 0) (Var 0))
+     (Clos (App (Var 0) (Var 0)) e :: e))).
+- rewrite frob_eq with (x:=bs omega e). simpl. rewrite frob_eq with (x:=bs delta e). simpl. rewrite Bind_On_Return. 
+rewrite Bind_On_Return. constructor. apply bisim_refl.
+- apply bisim_trans with (b:=(bs omega e)). apply bisim_symm in H. assumption. apply CIH.  Qed.
+
+
+ apply CIH.  
+rewrite frob_eq with (x:=(bs (App (Var 0) (Var 0)) (cons (Clos (App (Var 0) (Var 0)) e) e))).
+simpl.
+rewrite frob_eq with (x:=bs (Var 0) (cons (Clos (App (Var 0) (Var 0)) e) e)). simpl.
+rewrite Bind_On_Return. rewrite Bind_On_Return.  constructor. constructor.
+rewrite frob_eq with (x:=(bs (App (Var 0) (Var 0)) (cons (Clos (App (Var 0) (Var 0)) e) e))).
+simpl.
+rewrite frob_eq with (x:=bs (Var 0) (cons (Clos (App (Var 0) (Var 0)) e) e)). simpl.
+ rewrite Bind_On_Return. rewrite Bind_On_Return. 
+rewrite del
+assert (bisim (bs omega e) 
+(Step (bs (App (Var 0) (Var 0)) (Clos (App (Var 0) (Var 0)) e :: e)))).
+
+Eval compute in ( bs  (Const 2) nil).
+
+
+
+
+
+
+
 
